Delete Constant op from closLang
The original plan was to introduce large constants as closLang's
Constant op, but that plan changed once it became apparent that we
want to treat closed lambdas (Fn) as constants too. So the new plan is
to have clos_annotate discover the large constants by annotating the
existing ops. This means that the Constant op is no longer needed.

Progress on issue #803

compiler/backend/semantics/closSemScript.sml
@@ -156,18 +156,6 @@ Definition do_install_def:
        | _ => (Rerr(Rabort Rtype_error),s))
 End
 
-Definition make_const_def:
-  make_const (ConstInt i) = Number i ∧
-  make_const (ConstStr s) = ByteVector (MAP (n2w o ORD) (mlstring$explode s)) ∧
-  make_const (ConstWord64 w) = Word64 w ∧
-  make_const (ConstCons t cs) = Block t (MAP make_const cs)
-Termination
-  WF_REL_TAC ‘measure const_size’
-  \\ Induct_on ‘cs’ \\ rw []
-  \\ fs [const_size_def] \\ res_tac
-  \\ pop_assum (qspec_then ‘t’ assume_tac) \\ fs []
-End
-
 Definition do_app_def:
   do_app (op:closLang$op) (vs:closSem$v list) ^s =
     case (op,vs) of
@@ -183,7 +171,6 @@ Definition do_app_def:
     | (AllocGlobal,[]) =>
         Rval (Unit, s with globals := s.globals ++ [NONE])
     | (Const i,[]) => Rval (Number i, s)
-    | (Constant c,[]) => Rval (make_const c, s)
     | (Build p,[]) =>
         (case p of
          | [Str t] => Rval (ByteVector (MAP (n2w o ORD) (mlstring$explode t)), s)
