compiler/backend/proofs/clos_constantProofScript.sml
@@ -6,6 +6,18 @@ open preamble closLangTheory clos_to_bvlTheory closSemTheory;
 
 val _ = new_theory "clos_constantProof";
 
+Definition make_const_def:
+  make_const (ConstInt i) = Number i ∧
+  make_const (ConstStr s) = ByteVector (MAP (n2w o ORD) (mlstring$explode s)) ∧
+  make_const (ConstWord64 w) = Word64 w ∧
+  make_const (ConstCons t cs) = Block t (MAP make_const cs)
+Termination
+  WF_REL_TAC ‘measure const_size’
+  \\ Induct_on ‘cs’ \\ rw []
+  \\ fs [const_size_def] \\ res_tac
+  \\ pop_assum (qspec_then ‘t’ assume_tac) \\ fs []
+End
+
 (* naive implementation *)
 
 Definition make_part_def:
