compiler/backend/proofs/clos_knownProofScript.sml
@@ -817,10 +817,6 @@ Proof
       >- (first_x_assum match_mp_tac >> fs[] >> metis_tac[]))
   >- (rename [‘EqualConst’]
       \\ rw [] \\ fs [Boolv_def])
-  >- (rename [‘Constant’]
-      \\ rw [] \\ qid_spec_tac ‘c’
-      \\ ho_match_mp_tac make_const_ind
-      \\ fs [make_const_def,EVERY_MEM,MEM_MAP,PULL_EXISTS])
   >> dsimp[]
 QED
 
